[contain] this beast!

DListRef.fst
@@ -40,8 +40,8 @@ let empty_list #t =
 val getSome: (a:option 'a{isSome a}) -> (b:'a{a == Some b})
 let getSome a = Some?.v a
 
-unfold let (@) (a:ref 't) (h0:heap) = sel h0 a
-unfold let (^@) (a:option (ref 't){isSome a}) (h0:heap) = (getSome a) @ h0
+unfold let (@) (a:ref 't) (h0:heap{h0 `contains` a}) = sel h0 a
+unfold let (^@) (a:option (ref 't){isSome a}) (h0:heap{h0 `contains` (getSome a)}) = (getSome a) @ h0
 
 unfold let (.[]) (s:seq 'a) (n:nat{n < length s}) = index s n
 
@@ -63,8 +63,9 @@ logic
 let dlist_is_valid' (#t:Type) (h0:heap) (n:dlist t) : GTot Type0 =
   not_aliased n.flink n.blink
 
-logic
+// logic
 let dlist_is_valid (#t:Type) (h0:heap) (n:ref (dlist t)) : GTot Type0 =
+  h0 `contains` n /\
   dlist_is_valid' h0 (n@h0)
 
 unfold
@@ -82,12 +83,14 @@ let ( <| ) (#t:Type) (a:ref (dlist t)) (b: dlist t) : GTot Type0 =
 
 let ( =|> ) (#t:Type) (a:ref (dlist t)) (b:ref (dlist t)) : ST unit
     (requires (fun h0 ->
+         h0 `contains` a /\ h0 `contains` b /\
          not_aliased00 a b /\
          not_aliased0 b (a@h0).blink))
     (ensures (fun h1 _ h2 ->
          modifies (only a) h1 h2 /\
          dlist_is_valid h2 a /\
          (forall (f:dlist t -> Type0) x. {:pattern f (x@h2)}
+            h1 `contains` x /\
             f (x@h1) /\ not_aliased00 x a ==> f (x@h2)) /\
          (a@h1).p == (a@h2).p /\
          (a@h1).blink == (a@h2).blink /\
@@ -97,12 +100,14 @@ let ( =|> ) (#t:Type) (a:ref (dlist t)) (b:ref (dlist t)) : ST unit
 
 let ( <|= ) (#t:Type) (a:ref (dlist t)) (b:ref (dlist t)) : ST unit
     (requires (fun h0 ->
+         h0 `contains` a /\ h0 `contains` b /\
          not_aliased00 a b /\
          not_aliased0 a (b@h0).flink))
     (ensures (fun h1 _ h2 ->
          modifies (only b) h1 h2 /\
          dlist_is_valid h2 b /\
          (forall (f:dlist t -> Type0) x. {:pattern f (x@h2)}
+            h1 `contains` x /\
             f (x@h1) /\ not_aliased00 x b ==> f (x@h2)) /\
          a@h1 == a@h2 /\
          (b@h1).p == (b@h2).p /\
@@ -111,11 +116,12 @@ let ( <|= ) (#t:Type) (a:ref (dlist t)) (b:ref (dlist t)) : ST unit
   b := { !b with blink = Some a }
 
 let ( !=|> ) (#t:Type) (a:ref (dlist t)) : ST unit
-    (requires (fun _ -> True))
+    (requires (fun h0 -> h0 `contains` a))
     (ensures (fun h1 _ h2 ->
          modifies (only a) h1 h2 /\
          dlist_is_valid h2 a /\
          (forall (f:dlist t -> Type0) x. {:pattern f (x@h2)}
+            h1 `contains` x /\
             f (x@h1) /\ not_aliased00 x a ==> f (x@h2)) /\
          (a@h1).p == (a@h2).p /\
          (a@h1).blink == (a@h2).blink /\
@@ -123,11 +129,12 @@ let ( !=|> ) (#t:Type) (a:ref (dlist t)) : ST unit
   a := { !a with flink = None }
 
 let ( !<|= ) (#t:Type) (a:ref (dlist t)) : ST unit
-    (requires (fun _ -> True))
+    (requires (fun h0 -> h0 `contains` a))
     (ensures (fun h1 _ h2 ->
          modifies (only a) h1 h2 /\
          dlist_is_valid h2 a /\
          (forall (f:dlist t -> Type0) x. {:pattern f (x@h2)}
+            h1 `contains` x /\
             f (x@h1) /\ not_aliased00 x a ==> f (x@h2)) /\
          (a@h1).p == (a@h2).p /\
          (a@h2).flink == (a@h2).flink /\
@@ -138,9 +145,18 @@ unfold let (~.) (#t:Type) (a:t) : Tot (erased (seq t)) = hide (Seq.create 1 a)
 unfold let (^+) (#t:Type) (a:t) (b:erased (seq t)) : Tot (erased (seq t)) = elift2 Seq.cons (hide a) b
 
 logic
+let all_nodes_contained (#t:Type) (h0:heap) (h:dlisthead t) : GTot Type0 =
+  let nodes = reveal h.nodes in
+  (isSome h.lhead ==> h0 `contains` (getSome h.lhead)) /\
+  (isSome h.ltail ==> h0 `contains` (getSome h.ltail)) /\
+  (forall i. {:pattern (h0 `contains` nodes.[i])}
+     h0 `contains` nodes.[i])
+
+logic
 let flink_valid (#t:Type) (h0:heap) (h:dlisthead t) : GTot Type0 =
   let nodes = reveal h.nodes in
   let len = length nodes in
+  all_nodes_contained h0 h /\
   (forall i. {:pattern (nodes.[i]@h0 |> nodes.[i+1])}
      ((0 <= i /\ i < len - 1) ==>
       nodes.[i]@h0 |> nodes.[i+1]))
@@ -149,6 +165,7 @@ logic
 let blink_valid (#t:Type) (h0:heap) (h:dlisthead t) : GTot Type0 =
   let nodes = reveal h.nodes in
   let len = length nodes in
+  all_nodes_contained h0 h /\
   (forall i. {:pattern (nodes.[i-1] <| nodes.[i]@h0)}
      ((1 <= i /\ i < len) ==>
       nodes.[i-1] <| nodes.[i]@h0))
@@ -158,6 +175,7 @@ let dlisthead_ghostly_connections (#t:Type) (h0:heap) (h:dlisthead t) : GTot Typ
   let nodes = reveal h.nodes in
   let len = length nodes in
   let empty = (len = 0) in
+  all_nodes_contained h0 h /\
   ~empty ==> (
     h.lhead ==$ nodes.[0] /\
     h.ltail ==$ nodes.[len-1] /\
@@ -167,6 +185,7 @@ let dlisthead_ghostly_connections (#t:Type) (h0:heap) (h:dlisthead t) : GTot Typ
 logic
 let elements_dont_alias1 (#t:Type) (h0:heap) (h:dlisthead t) : GTot Type0 =
   let nodes = reveal h.nodes in
+  all_nodes_contained h0 h /\
   (forall i j. {:pattern (not_aliased (nodes.[i]@h0).flink (nodes.[j]@h0).flink)}
      0 < i /\ i < j /\ j < length nodes ==>
    not_aliased (nodes.[i]@h0).flink (nodes.[j]@h0).flink)
@@ -174,6 +193,7 @@ let elements_dont_alias1 (#t:Type) (h0:heap) (h:dlisthead t) : GTot Type0 =
 logic
 let elements_dont_alias2 (#t:Type) (h0:heap) (h:dlisthead t) : GTot Type0 =
   let nodes = reveal h.nodes in
+  all_nodes_contained h0 h /\
   (forall i j. {:pattern (not_aliased (nodes.[i]@h0).blink (nodes.[j]@h0).blink)}
      0 < i /\ i < j /\ j < length nodes ==>
    not_aliased (nodes.[i]@h0).blink (nodes.[j]@h0).blink)
@@ -186,6 +206,7 @@ let elements_dont_alias (#t:Type) (h0:heap) (h:dlisthead t) : GTot Type0 =
 logic
 let elements_are_valid (#t:Type) (h0:heap) (h:dlisthead t) : GTot Type0 =
   let nodes = reveal h.nodes in
+  all_nodes_contained h0 h /\
   (forall i. {:pattern (dlist_is_valid h0 nodes.[i])}
      dlist_is_valid h0 nodes.[i])
 
@@ -213,7 +234,7 @@ let test1 () : Tot unit = assert (forall h0 t. dlisthead_is_valid h0 (empty_list
 
 val singletonlist: #t:eqtype -> e:ref (dlist t) ->
   ST (dlisthead t)
-  (requires (fun _ -> True))
+  (requires (fun h0 -> h0 `contains` e))
   (ensures (fun h0 y h1 -> modifies (only e) h0 h1 /\ dlisthead_is_valid h1 y))
 let singletonlist #t e =
   !<|= e; !=|> e;
@@ -226,7 +247,10 @@ let member_of (#t:eqtype) (h0:heap) (h:dlisthead t) (e:ref (dlist t)) : GTot boo
   isSome r
 
 // logic : Cannot use due to https://github.com/FStarLang/FStar/issues/638
-let has_nothing_in (#t:eqtype) (h0:heap) (h:dlisthead t) (e:ref (dlist t)) : GTot Type0 =
+let has_nothing_in (#t:eqtype) (h0:heap)
+    (h:dlisthead t{dlisthead_is_valid h0 h})
+    (e:ref (dlist t){h0 `contains` e})
+  : GTot Type0 =
   (~(member_of h0 h e)) /\
   (not_aliased0 e h.lhead) /\
   (not_aliased0 e h.ltail) /\
@@ -245,6 +269,7 @@ type nonempty_dlisthead t = (h:dlisthead t{isSome h.lhead /\ isSome h.ltail})
 val dlisthead_make_valid_singleton: #t:eqtype -> h:nonempty_dlisthead t ->
   ST (dlisthead t)
     (requires (fun h0 ->
+         h0 `contains` (getSome h.lhead) /\
          isNone (h.lhead^@h0).flink /\ isNone (h.lhead^@h0).blink))
     (ensures (fun h1 y h2 -> modifies_none h1 h2 /\ dlisthead_is_valid h2 y))
 let dlisthead_make_valid_singleton #t h =
